We have,
$$
\begin{align}
a + b &= 39 \tag{1} \\

ab & = 324 \tag{2} \\ \\
\end{align}
$$
We know that,
$$
\begin{align}
(a - b)^2 &= a^2 + b^2 - 2ab \\
&= (a^2 + b^2 + 2ab) - 4ab \\
&= (a + b)^2 - 4ab \\
&= (39)^2 - 4(324) \tag{From (1) and (2)} \\
&= 225
\end{align}
$$
$$
\therefore~~~ a - b = \pm15 \tag{3}
$$
Adding eq (1) and (3),
$$
\begin{align}
a &= {39 \pm 15 \over 2} \\
&= 27, 12 \\
\\
\implies b &= 39 - a \tag{From (1)} \\
&= 12, 27
\end{align}
$$
Hence, either
$$
a = 27,~b = 12 \quad \text{or,} \quad a=12,~b=27
$$
